Soundness property formulation & proof

theories/ProofChecker.v
@@ -25,7 +25,7 @@ Definition validate_step
   (step : Step) (problem : ConstraintProblem) :=
   let inference := clausal_form step in
   match (inference_rule step) with
-  | rup_inf db => rup db inference
+  | rup_inf db => rup db (map atomic_not inference)
   | linear constraint => linear_checker inference constraint
   end.
 
@@ -38,6 +38,49 @@ Definition validate_conclusion
   (* end in *)
   (* existsb (fun cons => Constraint.eqb cons (nogood target)) (constraints problem). *)
 
+Definition append_inference (problem : ConstraintProblem) (step : Step) : ConstraintProblem :=
+  {|
+    variables := variables problem ;
+    constraints := (nogood (clausal_form step)) :: (constraints problem)
+  |}.
+
+Theorem append_soundness :
+  forall (problem : ConstraintProblem) (step : Step) (sol : Assignment),
+  Is_true (validate_step step problem) -> 
+  (
+    forall (constraint : Constraint), 
+    In constraint (constraints problem) ->
+    Is_true (satisfies_constraint constraint sol)
+  ) -> (
+    forall (constraint : Constraint), 
+    In constraint (constraints (append_inference problem step)) ->
+    Is_true (satisfies_constraint constraint sol)
+  ).
+Proof.
+  intros problem step sol Hval Hsat base_constraint Hin.
+  unfold append_inference in Hin.
+  simpl in Hin.
+  destruct Hin as [Enogood|Hin] ; try apply Hsat, Hin.
+  rewrite <- Enogood.
+  unfold satisfies_constraint.
+  unfold validate_step in Hval.
+  destruct (inference_rule step) eqn:Einference.
+  + apply Is_true_eq_true, linear_inference_checker_correct in Hval.
+    unfold is_valid_linear_inference in Hval.
+    apply Hval.
+    (* TODO Show that the listed constraint can be found in the original model *)
+    admit.
+  + apply Is_true_eq_true in Hval.
+    specialize valid_rup_on_negation with
+      (clause_seq := database) (nogood := clausal_form step).
+    unfold is_valid_nogood.
+    intros Hrup.
+    apply Hrup.
+    - apply Is_true_eq_left, Hval.
+    - (* TODO Show that all database clauses can be found in the model *)
+      admit.
+Admitted.
+
 Fixpoint validate_unpacked
   (proof_steps : list Step) (proof_conclusion : Conclusion)
   (problem : ConstraintProblem) : CheckerVerdict :=
@@ -49,11 +92,7 @@ Fixpoint validate_unpacked
     | step :: tail =>
         if validate_step step problem
         then
-        let problem_append :=
-        {|
-          variables := variables problem ;
-          constraints := (nogood (clausal_form step)) :: (constraints problem)
-        |} in
+        let problem_append := append_inference problem step in
         let tail_verdict := validate_unpacked tail proof_conclusion problem_append in
         inc_step_index tail_verdict
         else bad_step 0 step
@@ -78,7 +117,6 @@ Lemma unsat_no_invalid_step_implies_valid :
 Proof.
   unfold is_valid_conclusion, satisfies_conclusion, validate.
   intros proof problem Eunsat Evalid sol con Hin Hsat.
-  exfalso.
   generalize dependent sol.
   generalize dependent con.
   rewrite Eunsat in Evalid.
@@ -111,7 +149,36 @@ Lemma bound_validate_append :
     conclusion proof = optimal bound ->
     validate proof problem = valid ->
     is_valid_conclusion (conclusion proof) problem.
-  Admitted.
+Proof.
+  unfold is_valid_conclusion, satisfies_conclusion, validate.
+  intros proof problem bound Ebound Evalid sol con Hin Hsat.
+  rewrite Ebound.
+  generalize dependent sol.
+  generalize dependent con.
+  rewrite Ebound in Evalid.
+  generalize dependent problem.
+  induction (steps proof) as [|proof_head proof_tail IHproof].
+  - (* TODO No implementation of conclusion validation yet, skipping this part for now *)
+    admit.
+  - intros.
+    simpl in Evalid.
+    destruct (validate_step proof_head problem) eqn:Evalid_step_packed ;
+    simpl in Evalid ; inversion Evalid as [Etail].
+    unfold inc_step_index in Etail.
+    remember 
+    {|
+      variables := variables problem ;
+      constraints := (nogood (clausal_form proof_head)) :: (constraints problem)
+    |} as problem_append eqn:Eappend.
+    destruct (validate_unpacked proof_tail (optimal bound) problem_append) eqn:Evalid_step ; inversion Etail.
+    apply IHproof with (problem := problem_append) (sol := sol) (con := con).
+    + apply Evalid_step.
+    + rewrite Eappend.
+      simpl.
+      right.
+      apply Hin.
+    + apply Hsat.
+Admitted.
 
 Theorem no_invalid_step_implies_valid :
   forall (proof : Proof) (problem : ConstraintProblem),
